% Preamble
\documentclass[a4paper, 12pt]{article}
\usepackage{titlesec}
\usepackage[margin=1in]{geometry}
\usepackage{pdfpages}
\usepackage{amssymb}
\newcommand{\qed}{\\\ensuremath{\\\blacksquare\pagebreak}}
\renewcommand{\b}[1]{\textbf{#1}}
\newcommand{\axiom}[1]{~\b{(Axiom #1)}}
\renewcommand{\d}{\\\ensuremath{\Downarrow\\~}}
\titlelabel{\thetitle.\quad}

% Document
\begin{document}


% Title Page
\begin{titlepage}
    %\includepdf{title.pdf}
\end{titlepage}

% 1
\section{What requirements S must fullfil in order to become a field?}
In order to show that $S$ is a field, we'll need to prove the following \textit{\textbf{binary operator}} properties:
\begin{enumerate}
    \item In $S$, there are two members, zero - $0_S$ and one - $1_S$
    \item $S$ supports the addition and multiplication binary operators
    \item Every member in $S$ can be negated, i.e. for every $x$ there is $-x$
    \item For every member in $S$ that is not $0_S$, $\exists{x^{-1}}\in{S}$, it is called the multiplicative inverse of $x$
\end{enumerate}
In addition, the mentioned binary operators should satisfy the following properties, referred to as \textit{\textbf{field axioms}}:
\begin{enumerate}
    \item Associativity of addition(A1) and multiplication(M1):
        $$ a+(b+c)=(a+b)+c $$
        $$ a\cdot(b\cdot{c})=(a\cdot{b})\cdot{c} $$
    \item Commutativity of addition(A2) and multiplication(M2):
        $$ a+b = b+a $$
        $$ a\cdot{b} = b\cdot{a} $$
    \item Additive identity(A3) and multiplicative identity(M3)
        $$ a+0=a $$
        $$ a\cdot{1}=a $$
    \item Additive inverse(A4) and multiplicative inverse(M4)
        $$ a + (-a) = 0 $$
        $$ a \cdot a^-1 = 1 $$
    \item Distributivity(D)
        $$ a(b + c) = (a \cdot{b})+(a \cdot{c}) $$
\end{enumerate}
\pagebreak

% 2
\section{Prove: $ ((a + b) + c) + d = (a + b) + (c + d) = a + (b + (c + d)) $}
\subsection{$ \underline{((a+b)+c)+d=(a+b)+(c+d)}: $}
let $h=(a+b)$\\
$(h+c)+d=((a+b)+c)+d$\\
$(h+c)+d = h+(c+d)$ \textbf{(Axiom A1)}\\
$ h+(c+d) = (a+b)+(c+d) $
\d
$((a+b)+c)+d=(a+b)+(c+d)$
\subsection{$ \underline{ a+(b+(c+d))=(a+b)+(c+d) }: $}
let $h=(c+d)$\\
$ a+(b+h) = a+(b+(c+d)) $\\
$ a+(b+h) = (a+b)+h $ \textbf{(Axiom A1)}\\
$ (a+b)+h = (a+b)+(c+d) $
\d
$ a+(b+(c+d)) = (a+b)+(c+d) $
\qed

% 3
\section{Prove: $ \forall{x,y}\in{F},~x(y-z) = xy-xz $}
$ x(y-z) = x(y+(-z)) $ \textbf{(Axiom A1)}\\
$ x(y+(-z)) = (x\cdot{y})+(x\cdot(-z))$ \textbf{(Axiom D)}\\
$ (x\cdot{y})+(x\cdot(-z)) = (x\cdot{y})+(-x\cdot{z})) = (x\cdot{y})-(x\cdot{z})) $\\
$ (x\cdot{y})-(x\cdot{z})) = xy - xz $
\qed

% 4
\section{Prove: $ \forall{x,y}\in{F},~ (x+y)(x+y) = xx + xy + yx + yy $}
let $ h=(x+y) $\\
$
    (x+y)(x+y) = h\cdot(x+y)\\
    h\cdot(x+y) = (x\cdot{h})+(y\cdot{h}) = x(x+y) + y(x+y) \axiom{D}\\
    x(x+y) + y(x+y) = \b{xx + xy + yx + yy} \axiom{D}
$
\qed

\end{document}