% Preamble
\documentclass[a4paper, 12pt]{article}
\usepackage[margin=1in]{geometry} % Set margin
\usepackage{pdfpages} % Insert pdf pages
\usepackage{amssymb,amsmath,amsthm, amsfonts} % Math libraries


% Custom commands
\newcommand{\sub}[1]{\subsection{\underline{#1}}}
\newcommand{\subsub}[1]{\subsubsection{\underline{#1}}}
\newcommand{\?}{\stackrel{?}{=}}
\newcommand{\R}{\ensuremath{\mathbb{R}}}
\newcommand{\F}{\ensuremath{\mathbb{F}}}
\newcommand{\eqbcuz}[1]{\text{~$\stackrel{(#1)}{=}$~}}
\renewcommand{\qed}{$$\blacksquare$$}
\renewcommand{\b}[1]{\textbf{#1}}
\renewcommand{\because}[1]{~\b{(#1)}\\}
\renewcommand{\d}{\ensuremath{\Downarrow\\~}}

% Begin Document %
\begin{document}

% Title Page
\begin{titlepage}
    \includepdf{title.pdf}
\end{titlepage}

% 2
\setcounter{section}{1}
\section{Prove: $ ((a + b) + c) + d = (a + b) + (c + d) = a + (b + (c + d)) $}

\sub{$((a+b)+c)+d=(a+b)+(c+d)$:}
First of all, we'll take a look at the left side of the equation.\\
We'll mark: $$h=(a+b)$$
Therefore: $$(h+c)+d=((a+b)+c)+d$$
$$(h+c)+d \eqbcuz{A1} h+(c+d) $$
We'll subtitue $h$ with $(a+b)$: $$ h+(c+d) = (a+b)+(c+d) $$
$$\d$$
$$((a+b)+c)+d=(a+b)+(c+d)$$

\sub{$a+(b+(c+d))=(a+b)+(c+d)$:}
We'll mark: $$h=(c+d)$$
Therefore: $$ a+(b+h) = a+(b+(c+d)) $$
$$ a+(b+h) \eqbcuz{A1} (a+b)+h $$
We'll subtitue $h$ with $(c+d)$: $$ (a+b)+h = (a+b)+(c+d) $$
$$\d$$
$$ a+(b+(c+d)) = (a+b)+(c+d) $$
\qed

% 8
\setcounter{section}{7}
\section{Is $B$ a field?}
    If $B$ fulfills all 9 field's axioms, $B$ is a field, let's check them one by one.
    \sub{A1 - Additive Associativity}
        $$ \bigg{[}\dbinom{a}{b}\oplus{}\dbinom{c}{d}\bigg{]}\oplus{}\dbinom{e}{f} \? \dbinom{a}{b} \oplus{} \bigg{[}\dbinom{c}{d}\oplus{}\dbinom{e}{f}\bigg{]} $$
        $$ \dbinom{a+c}{b+d}\oplus{}\dbinom{e}{f} \? \dbinom{a}{b} \oplus{} \dbinom{c+e}{d+f} $$
        $$ \dbinom{a+c+e}{b+d+f} = \dbinom{a+c+e}{b+d+f} $$

    \sub{M1 - Multiplicative Associativity}
        $$ \bigg{[}\dbinom{a}{b}\odot{}\dbinom{c}{d}\bigg{]}\odot{}\dbinom{e}{f} \? \dbinom{a}{b} \odot{} \bigg{[}\dbinom{c}{d}\odot{}\dbinom{e}{f}\bigg{]} $$
        $$ \dbinom{ac}{bd}\odot{}\dbinom{e}{f} \? \dbinom{a}{b} \odot{} \dbinom{ce}{df} $$
        $$ \dbinom{ace}{bdf} = \dbinom{ace}{bdf} $$

    \sub{A2 - Additive Commutativity}
        $$ \dbinom{a}{b} \oplus \dbinom{c}{d} \? \dbinom{c}{d} \oplus \dbinom{a}{b} $$
        $$ \dbinom{a+c}{b+d} \? \dbinom{c+a}{d+b} $$
        As $a,b \in {\R}$, we can use axiom A2:
        $$ \dbinom{a+c}{b+d} = \dbinom{c+a}{d+b} $$

    \sub{M2 - Multiplicative Commutativity}
        $$ \dbinom{a}{b} \odot \dbinom{c}{d} \? \dbinom{c}{d} \odot \dbinom{a}{b} $$
        $$ \dbinom{ac}{bd} \? \dbinom{ca}{db} $$
        As $a,b,c,d \in {\R}$, we can use axiom M2:
        $$ \dbinom{ac}{bd} = \dbinom{ca}{db} $$

    \sub{A3 - Additive Identity}
        Now, we'll look for $0_{B}$:
        $$ \dbinom{a}{b}\oplus\dbinom{0}{0} = \dbinom{a+0}{b+0} $$
        As $a,b \in {\R}$, we can use axiom A3:
        $$ \dbinom{a+0}{b+0} = \dbinom{a}{b} $$
        Therefore:
        $$ \dbinom{0}{0} = 0_{B} $$
    
    \sub{M3 - Multiplicative Identity}
        Now, we'll look for $1_{B}$:
        $$ \dbinom{a}{b}\odot\dbinom{1}{1} = \dbinom{1a}{1b} $$
        As $a,b \in {\R}$, we can use axiom M3:
        $$ \dbinom{1a}{1b} = \dbinom{a}{b} $$ 
        Therefore:
        $$ \dbinom{1}{1} = 1_{B} $$
        This answers (\textit{ii}).

    \sub{A4 - Additive Inverse}
        Now, let us find if exists a member, $\dbinom{c}{d} \in{B}$, for any other member $\dbinom{a}{b} \in{B}$, so that:
        $$ \dbinom{a}{b}\oplus\dbinom{c}{d} = 0_{B} $$
        We'll start by adding the inverse of every number to itself:
        $$\dbinom{a}{b}\oplus\dbinom{-a}{-b} = \dbinom{a+(-a)}{b+(-b)} $$
        As $a,b \in {\R}$, we can use axiom A4 to find the sum's value:
        $$ \dbinom{a+(-a)}{b+(-b)} =\dbinom{0}{0}=0_{B} $$
        This answers (\textit{i}).
        \pagebreak

    \sub{M4 - Multiplicative Inverse}
        Now, let us find if exists a member, $\dbinom{c}{d} \in{B}$, for any other member $\dbinom{a}{b} \in{B}$, so that:
        $$ \dbinom{a}{b}\odot\dbinom{c}{d} = 1_{B} $$
        Let's multiply every number by its multiplicitive inverse:
        $$ \dbinom{a}{b}\odot\dbinom{\frac{1}{a}}{\frac{1}{b}}=\dbinom{a\cdot{\frac{1}{a}}}{b\cdot{\frac{1}{b}}} $$
        As $a,b \in {\R}$, we can use axiom M4:
        $$ \dbinom{a\cdot{\frac{1}{a}}}{b\cdot{\frac{1}{b}}} = \dbinom{1}{1} $$
        $$ \dbinom{1}{1} = 1_{B} $$

    \sub{D - Distributivity}
    In order to display distributivity, we'll need to show the $B$ equivalent of:
    $$ a\cdot{(b+c)}=a\cdot{b}+a\cdot{c} $$
    i.e., we need to prove:
    $$ \dbinom{a}{b} \odot \bigg{[} \dbinom{c}{d} \oplus \dbinom{e}{f} \bigg{]} = \dbinom{ac}{bd} \oplus \dbinom{ae}{bf} $$
    First, let's solve: $$ \bigg{[} \dbinom{c}{d} \oplus \dbinom{e}{f} \bigg{]} $$
    We use $B$'s binary additive operator:
    $$ \dbinom{c}{d} \oplus \dbinom{e}{f} = \dbinom{c+e}{d+f} $$
    We use $B$'s binary multiplicative operator: $$ \dbinom{a}{b} \odot \dbinom{c+e}{d+f} = \dbinom{a(c+e)}{b(d+f)} $$
    As $a,b,c,d,e,f \in {\R}$, we can use the distributivity axiom to unpack:
    $$ \dbinom{a(c+e)}{b(d+f)} = \dbinom{ac+ae}{bd+bf} = \dbinom{ac}{bd} \oplus \dbinom{ae}{bf} $$
    This answers (\textit{iii}).
    \qed
    \pagebreak

\setcounter{section}{22}
\section{Prove $-(a+b)=(-a)+(-b)=-a-b$:}
According to axiom \textit{A4}: $$ -(a+b) + (a+b) = 0$$
Now, let's add $-a-b$ to both sides of the equation: $$ -(a+b)+(a+b)-a-b=-a-b $$
And use axioms \textit{A1} and \textit{A2}: $$ -(a+b)+(a+(-a))+(b+(-b))=-a-b $$
According to axiom \textit{A4}: $$ -(a+b)+(0)+(0)=-a-b $$
And according to axiom \textit{A3} and the definition of deduction: $$ -(a+b)=-a-b=(-a)+(-b) $$
\qed

\setcounter{section}{25}
\section{Prove $ (-a)(-b) = ab $:}
According to multiplicative identity axiom: $$ (-a)(-b) = ((-1)\cdot{a})((-1)\cdot{b}) $$
According to multiplicative commutativity axiom: $$ ((-1)\cdot{a})((-1)\cdot{b}) = (-1)\cdot(-1)\cdot{a}\cdot{b} $$
And multiplicative identity axiom again: $$ (-1)\cdot(-1)\cdot{a}\cdot{b} = 1 \cdot{a} \cdot{b} = ab $$
\qed\pagebreak

\setcounter{section}{29}
\section{Prove $a\neq{0} \Longrightarrow 0/a=0$:}
\sub{Lemma: $ a\cdot{0} = 0 $}
According to the distributivity and multiplicative identity axioms: $$ a\cdot{0}+a = a(0+1) = a\cdot{1} = a $$
Therefore: $$ a\cdot{0}+a = a $$
We'll subtract $a$ from both sides of the equation: $$ a\cdot{0} + a - a = a - a $$
$$ a\cdot{0} = 0 $$
\qed

\sub{$a\neq{0} \Longrightarrow 0/a=0$}
According to the definition of division: $$ 0/a = 0\cdot{a^{-1}} $$
According to the lemma: $$ 0\cdot{a^{-1}} = 0 $$
\qed

\setcounter{section}{36}
\section{Solve in \R:$$ \sum_{i=1}^{53}{(-1)^i} $$}
We can notice that 53 is an odd number, and therefore $(-1)$ is multiplied by itself an odd number of times.\\
Therefore, we can say that the following two are identical: $$ \sum_{i=1}^{53}{(-1)^i} = \sum_{i=1}^{1}{(-1)^i} = -1 $$
\qed\pagebreak

\section{Solve in \R:$$ \sum_{k=3}^{20}{[k\cdot{k}-(k-1)\cdot(k-1)]} $$}
First, let's understand this by solving: $$ \sum_{k=3}^{4}{[k\cdot{k}-(k-1)\cdot(k-1)]} $$
$$ \sum_{k=3}^{4}{[k\cdot{k}-(k-1)\cdot(k-1)]} = 4^2 -3^2 + 3^2 -2^2  = 4^2 - 2^2$$
Therefore, we can extrapolate:
$$ \sum_{k=3}^{20}{[k\cdot{k}-(k-1)\cdot(k-1)]} = 20^2 - 2^2$$
\qed

\setcounter{section}{48}
\section{$$ a_1X_1 +  a_2X_2+ a_3X_3 = b$$}
\sub{$(1,1,2,1)$:}
First, we'll apply the coefficients:
$$ X_1 +  X_2+ 2X_3 = 1 $$
Change the equation to a single variable equation:
$$ X_1 = 1 - t_2 - 2t_3 $$
Therefore: $$
\mathbb{S} = \Bigg{\{}
    \bordermatrix {
    &        \cr
    & 1 - t_2 - 2t_3    \cr
    & t_2    \cr
    & t_3    \cr
    }
:
t_2, t_3 \in {\R}
\Bigg{\}} $$

\sub{$(0,1,6,3)$:}
First, we'll apply the coefficients:
$$ 0X_1 +  X_2+ 6X_3 = 3 $$
Change the equation to a single variable equation:
$$ X_2 = 3-0t_1-6t_3 = 3-6t_3 $$
Therefore: $$
\mathbb{S} = \Bigg{\{}
    \bordermatrix {
    &        \cr
    & t_1    \cr
    & 3-6t_3    \cr
    & t_3    \cr
    }
:
t_1, t_3 \in {\R}
\Bigg{\}} $$

\sub{$(0,3,6,3)$:}
First, we'll apply the coefficients:
$$ 0X_1 +  3X_2+ 6X_3 = 3 $$
We'll divide both sides of the equation by $3$: $$ 0X_1 +  X_2+ 2X_3 = 1 $$
Change the equation to a single variable equation: $$ X_2 = 1 - 0t_1 - 2t_3 = 1-2t_3 $$
Therefore: $$
\mathbb{S} = \Bigg{\{}
    \bordermatrix {
    &        \cr
    & t_1    \cr
    & 1-2t_3    \cr
    & t_3    \cr
    }
:
t_1, t_3 \in {\R}
\Bigg{\}} $$
\qed

% End Document %
\end{document}